ebpf/Asm.v
@@ -17,13 +17,20 @@ Require Import Maps Values Memory.
 Require Import Globalenvs.
 Require Import Locations.
 
+Require Import Conventions Events Smallstep.
+Require Stacklayout.
+
 (** * Abstract syntax *)
 
-(** Integer registers. *)
+(** Registers. *)
 
 Inductive ireg: Type := R0 | R1 | R2 | R3 | R4 | R5 | R6 | R7 | R8 | R9 | R10.
+Inductive freg: Type := F0 | F1 | F2.
 
 Lemma ireg_eq: forall (x y: ireg), {x=y} + {x<>y}.
+Proof. decide equality. Defined.
+
+Lemma freg_eq: forall (x y: freg), {x=y} + {x<>y}.
 Proof. decide equality. Defined.
 
 
@@ -31,39 +38,39 @@ Proof. decide equality. Defined.
 
 Inductive preg :=
 | IR : ireg -> preg  (**r integer registers *)
+| FR : freg -> preg  (**r float registers, not available in eBPF *)
 | PC : preg          (**r program counter *)
 | RA : preg.         (**r pseudo-reg representing return address *)
 
 Coercion IR: ireg >-> preg.
+Coercion FR: freg >-> preg.
 
-Lemma reg_eq: forall (x y: preg), {x=y} + {x<>y}.
-Proof. decide equality. apply ireg_eq.
+Lemma preg_eq: forall (x y: preg), {x=y} + {x<>y}.
+Proof. decide equality. apply ireg_eq. apply freg_eq.
 Defined.
 
-Module RegEq.
+Module PregEq.
   Definition t  := preg.
-  Definition eq := reg_eq.
-End RegEq.
+  Definition eq := preg_eq.
+End PregEq.
 
-Module Regmap := EMap(RegEq).
+Module Pregmap := EMap(PregEq).
 
 
 (** Translation of the LTL/Linear/Mach view of machine registers
   to the eBPF view. *)
 
-Definition preg_of (r: mreg) : option preg :=
+Definition preg_of (r: mreg) : preg :=
   match r with
-  | I0 => Some (IR R0) | I1 => Some (IR R1) | I2 => Some (IR R2)
-  | I3 => Some (IR R3) | I4 => Some (IR R4) | I5 => Some (IR R5)
-  | I6 => Some (IR R6) | I7 => Some (IR R7) | I8 => Some (IR R8)
-  | I9 => Some (IR R9)
-  | D0 | D1 | D2 => None
-  end.
+  | I0 => IR R0 | I1 => IR R1 | I2 => IR R2 | I3 => IR R3 | I4 => IR R4
+  | I5 => IR R5 | I6 => IR R6 | I7 => IR R7 | I8 => IR R8 | I9 => IR R9
 
+  | D0 => FR F0 | D1 => FR F1 | D2 => FR F2
+  end.
 
 (** Conventional names for stack pointer ([SP]) *)
 
-Notation "'SP'" := (IR R10) (only parsing) : asm.
+Notation "'SP'" := R10 (only parsing) : asm.
 
 
 (** The instruction set.  Most instructions correspond exactly to
@@ -102,17 +109,18 @@ Inductive cmpOp : Type :=
   | LE: signedness -> cmpOp. (**r e1 <= e2 *)
 
 Inductive sizeOp : Type :=
-  | Byte      (**r 1 byte *)
-  | HalfWord  (**r 2 bytes *)
-  | Word.     (**r 4 bytes *)
+  | Byte        (**r 1 byte *)
+  | HalfWord    (**r 2 bytes *)
+  | Word        (**r 4 bytes *)
+  | SignedWord. (**r 4 bytes (signed) *)
 
 Inductive instruction : Type :=
-  | Pload : sizeOp -> preg -> preg -> off -> instruction        (**r dereference load *)
-  | Pstore : sizeOp -> preg -> preg+imm -> off -> instruction   (**r dereference store *)
-  | Palu : aluOp -> preg -> preg+imm -> instruction             (**r arithmetics *)
-  | Pcmp : cmpOp -> preg -> preg+imm -> instruction             (**r comparison without branching: eBPF extension *)
+  | Pload : sizeOp -> ireg -> ireg -> off -> instruction        (**r dereference load *)
+  | Pstore : sizeOp -> ireg -> ireg+imm -> off -> instruction   (**r dereference store *)
+  | Palu : aluOp -> ireg -> ireg+imm -> instruction             (**r arithmetics *)
+  | Pcmp : cmpOp -> ireg -> ireg+imm -> instruction             (**r comparison without branching: eBPF extension *)
   | Pjmp : ident+label -> instruction                           (**r unconditional jump *)
-  | Pjmpcmp : cmpOp -> preg -> preg+imm -> label -> instruction (**r conditional jump with comparison *)
+  | Pjmpcmp : cmpOp -> ireg -> ireg+imm -> label -> instruction (**r conditional jump with comparison *)
   | Pcall : ident -> signature -> instruction                   (**r function call *)
   | Pret : instruction                                          (**r function return *)
 
@@ -120,8 +128,8 @@ Inductive instruction : Type :=
   | Plabel (lbl: label)                                         (**r define a code label *)
   | Pbuiltin: external_function -> list (builtin_arg preg)
               -> builtin_res preg -> instruction                (**r built-in function (pseudo) *)
-  | Pallocframe (sz: Z) (pos: ptrofs)                           (**r allocate new stack frame *)
-  | Pfreeframe  (sz: Z) (pos: ptrofs).                          (**r deallocate stack frame and restore previous frame *)
+  | Pallocframe (sz: Z) (ofs_ra ofs_link: ptrofs)               (**r allocate new stack frame *)
+  | Pfreeframe  (sz: Z) (ofs_ra ofs_link: ptrofs).              (**r deallocate stack frame and restore previous frame *)
 
 
 Definition code := list instruction.
@@ -137,15 +145,48 @@ Definition program := AST.program fundef unit.
   type [Tint], float registers to values of type [Tfloat],
   and condition bits to either [Vzero] or [Vone]. *)
 
-Definition regset := Regmap.t val.
+Definition regset := Pregmap.t val.
 Definition genv := Genv.t fundef unit.
 
 Notation "a # b" := (a b) (at level 1, only parsing) : asm.
-Notation "a # b <- c" := (Regmap.set b c a) (at level 1, b at next level) : asm.
+Notation "a # b <- c" := (Pregmap.set b c a) (at level 1, b at next level) : asm.
 
 Open Scope asm.
 
+(** Undefining some registers *)
+
+Fixpoint undef_regs (l: list preg) (rs: regset) : regset :=
+  match l with
+  | nil => rs
+  | r :: l' => undef_regs l' (rs#r <- Vundef)
+  end.
+
+(** Assigning a register pair *)
+
+Definition set_pair (p: rpair preg) (v: val) (rs: regset) : regset :=
+  match p with
+  | One r => rs#r <- v
+  | Twolong rhi rlo => rs#rhi <- (Val.hiword v) #rlo <- (Val.loword v)
+  end.
+
+(** Assigning the result of a builtin *)
+
+Fixpoint set_res (res: builtin_res preg) (v: val) (rs: regset) : regset :=
+  match res with
+  | BR r => rs#r <- v
+  | BR_none => rs
+  | BR_splitlong hi lo => set_res lo (Val.loword v) (set_res hi (Val.hiword v) rs)
+  end.
+
 Section RELSEM.
+
+(** Looking up instructions in a code sequence by position. *)
+
+Fixpoint find_instr (pos: Z) (c: code) {struct c} : option instruction :=
+  match c with
+  | nil => None
+  | i :: il => if zeq pos 0 then Some i else find_instr (pos - 1) il
+  end.
 
 (** Position corresponding to a label *)
 
@@ -200,7 +241,7 @@ Definition goto_label (f: function) (lbl: label) (rs: regset) (m: mem) :=
       end
   end.
 
-Definition eval_reg_imm (rs : regset) (ri: preg+imm) : val :=
+Definition eval_reg_imm (rs : regset) (ri: ireg+imm) : val :=
   match ri with
   | inl r => rs#r
   | inr i => Vint i
@@ -227,9 +268,9 @@ Definition eval_alu (b: aluOp) (v1 v2: val) : option val :=
 
 (** Evaluation of [Pcmp] and [Pjmpcmp] operands *)
 
-Definition eval_cmp (op: cmpOp) (rs: regset) (m: mem) (r: preg) (ri: preg+imm) : option bool :=
+Definition eval_cmp (op: cmpOp) (rs: regset) (m: mem) (r: ireg) (ri: ireg+imm) : option bool :=
   match op with
-  | EQ          => Val.cmp_bool Ceq (rs#r) (eval_reg_imm rs ri)
+  | EQ          => Val.cmpu_bool (Mem.valid_pointer m) Ceq (rs#r) (eval_reg_imm rs ri)
   | GT Signed   => Val.cmp_bool Cgt (rs#r) (eval_reg_imm rs ri)
   | GT Unsigned => Val.cmpu_bool (Mem.valid_pointer m) Cgt (rs#r) (eval_reg_imm rs ri)
   | GE Signed   => Val.cmp_bool Cge (rs#r) (eval_reg_imm rs ri)
@@ -238,8 +279,8 @@ Definition eval_cmp (op: cmpOp) (rs: regset) (m: mem) (r: preg) (ri: preg+imm) :
   | LT Unsigned => Val.cmpu_bool (Mem.valid_pointer m) Clt (rs#r) (eval_reg_imm rs ri)
   | LE Signed   => Val.cmp_bool Cle (rs#r) (eval_reg_imm rs ri)
   | LE Unsigned => Val.cmpu_bool (Mem.valid_pointer m) Cle (rs#r) (eval_reg_imm rs ri)
-  | SET         => Val.cmp_bool Cne (Val.and (rs#r) (eval_reg_imm rs ri)) (Vint Int.zero)
-  | NE          => Val.cmp_bool Cne (rs#r) (eval_reg_imm rs ri)
+  | SET         => Val.cmpu_bool (Mem.valid_pointer m) Cne (Val.and (rs#r) (eval_reg_imm rs ri)) (Vint Int.zero)
+  | NE          => Val.cmpu_bool (Mem.valid_pointer m) Cne (rs#r) (eval_reg_imm rs ri)
   end.
 
 
@@ -250,25 +291,29 @@ Definition size_to_memory_chunk (size: sizeOp) : memory_chunk :=
   | Byte => Mint8unsigned
   | HalfWord => Mint16unsigned
   | Word => Many32
+  | SignedWord => Mint32
   end.
 
-Definition exec_load (k: sizeOp) (r:preg) (r':preg) (o:Ptrofs.int) (rs: regset) (m:mem) :=
+Definition exec_load (k: sizeOp) (r:ireg) (r':ireg) (o:Ptrofs.int) (rs: regset) (m:mem) :=
   match Mem.loadv (size_to_memory_chunk k) m (Val.offset_ptr rs#r' o) with
   | None => Stuck
   | Some v => Next (nextinstr (rs#r <- v)) m
   end.
 
-Definition exec_store (k: sizeOp) (r:preg) (ri:preg+imm) (o:Ptrofs.int) (rs: regset) (m:mem) :=
+Definition exec_store (k: sizeOp) (r:ireg) (ri:ireg+imm) (o:Ptrofs.int) (rs: regset) (m:mem) :=
   match Mem.storev (size_to_memory_chunk k) m (Val.offset_ptr rs#r o) (eval_reg_imm rs ri) with
   | None => Stuck
   | Some m' => Next (nextinstr rs) m'
   end.
 
-Definition exec_alu (o: aluOp)  (r: preg) (ri: preg+imm) (rs: regset) (m: mem) :=
+Definition exec_alu (o: aluOp)  (r: ireg) (ri: ireg+imm) (rs: regset) (m: mem) :=
   match eval_alu o (rs#r) (eval_reg_imm rs ri) with
   | None => Stuck
   | Some v => Next (nextinstr (rs#r <- v)) m
   end.
+
+Definition exec_cmp (r: ireg) (rs: regset) (m: mem) (res: option bool) :=
+  Next (nextinstr (rs#r <- (Val.of_optbool res))) m.
 
 Definition exec_branch (f: function) (l: label) (rs: regset) (m: mem) (res: option bool) : outcome :=
   match res with
@@ -290,7 +335,7 @@ Definition exec_instr (f: function) (i: instruction) (rs:regset) (m: mem) : outc
   | Pload k r r' o   => exec_load k r r' o rs m
   | Pstore k r ri o  => exec_store k r ri o rs m
   | Palu o r ri      => exec_alu o r ri rs m
-  | Pcmp o r ri      => Next (rs#r <- (Val.of_optbool (eval_cmp o rs m r ri))) m
+  | Pcmp o r ri      => exec_cmp r rs m (eval_cmp o rs m r ri)
   | Pjmp (inl l)     => goto_label f l rs m
   | Pjmp (inr id)    => Next (rs#PC <- (Genv.symbol_address ge id Ptrofs.zero)) m
   | Pjmpcmp o r ri l => exec_branch f l rs m (eval_cmp o rs m r ri)
@@ -298,8 +343,205 @@ Definition exec_instr (f: function) (i: instruction) (rs:regset) (m: mem) : outc
                                 #PC <- (Genv.symbol_address ge s Ptrofs.zero)
                           ) m
   | Pret             => Next (rs#PC <- (rs#RA)) m
+
+  (** Pseudo-instructions *)
+  | Pallocframe sz ofs_ra ofs_link =>
+      let (m1, stk) := Mem.alloc m 0 sz in
+      let sp := (Vptr stk Ptrofs.zero) in
+      match Mem.storev Mptr m1 (Val.offset_ptr sp ofs_link) rs#SP with
+      | None => Stuck
+      | Some m2 =>
+          match Mem.storev Mptr m2 (Val.offset_ptr sp ofs_ra) rs#RA with
+          | None => Stuck
+          | Some m3 => Next (nextinstr (rs #R0 <- (rs#SP) #SP <- sp)) m3
+          end
+      end
+
+  | Pfreeframe sz ofs_ra ofs_link =>
+      match Mem.loadv Mptr m (Val.offset_ptr rs#SP ofs_ra) with
+      | None => Stuck
+      | Some ra =>
+          match Mem.loadv Mptr m (Val.offset_ptr rs#SP ofs_link) with
+          | None => Stuck
+          | Some sp =>
+              match rs#SP with
+              | Vptr stk ofs =>
+                  match Mem.free m stk 0 sz with
+                  | None => Stuck
+                  | Some m' => Next (nextinstr (rs#SP <- sp #RA <- ra)) m'
+                  end
+              | _ => Stuck
+              end
+          end
+      end
+
   | Plabel l         => Next (nextinstr rs) m
+
   | _                => Stuck
   end.
 
+(** Undefine all registers except SP and callee-save registers *)
+
+Definition undef_caller_save_regs (rs: regset) : regset :=
+  fun r =>
+    if preg_eq r SP
+    || In_dec preg_eq r (List.map preg_of (List.filter is_callee_save all_mregs))
+    then rs r
+    else Vundef.
+
+(** Extract the values of the arguments of an external call.
+    We exploit the calling conventions from module [Conventions], except that
+    we use eBPF registers instead of locations. *)
+
+Inductive extcall_arg (rs: regset) (m: mem): loc -> val -> Prop :=
+  | extcall_arg_reg: forall r,
+      extcall_arg rs m (R r) (rs (preg_of r))
+  | extcall_arg_stack: forall ofs ty bofs v,
+      bofs = Stacklayout.fe_ofs_arg + 4 * ofs ->
+      Mem.loadv (chunk_of_type ty) m
+                (Val.offset_ptr rs#SP (Ptrofs.repr bofs)) = Some v ->
+      extcall_arg rs m (S Outgoing ofs ty) v.
+
+Inductive extcall_arg_pair (rs: regset) (m: mem): rpair loc -> val -> Prop :=
+  | extcall_arg_one: forall l v,
+      extcall_arg rs m l v ->
+      extcall_arg_pair rs m (One l) v
+  | extcall_arg_twolong: forall hi lo vhi vlo,
+      extcall_arg rs m hi vhi ->
+      extcall_arg rs m lo vlo ->
+      extcall_arg_pair rs m (Twolong hi lo) (Val.longofwords vhi vlo).
+
+Definition extcall_arguments
+    (rs: regset) (m: mem) (sg: signature) (args: list val) : Prop :=
+  list_forall2 (extcall_arg_pair rs m) (loc_arguments sg) args.
+
+Definition loc_external_result (sg: signature) : rpair preg :=
+  map_rpair preg_of (loc_result sg).
+
+(** Execution of the instruction at [rs PC]. *)
+
+Inductive state: Type :=
+  | State: regset -> mem -> state.
+
+Inductive step: state -> trace -> state -> Prop :=
+  | exec_step_internal:
+      forall b ofs f i rs m rs' m',
+      rs PC = Vptr b ofs ->
+      Genv.find_funct_ptr ge b = Some (Internal f) ->
+      find_instr (Ptrofs.unsigned ofs) (fn_code f) = Some i ->
+      exec_instr f i rs m = Next rs' m' ->
+      step (State rs m) E0 (State rs' m')
+  | exec_step_builtin:
+      forall b ofs f ef args res rs m vargs t vres rs' m',
+      rs PC = Vptr b ofs ->
+      Genv.find_funct_ptr ge b = Some (Internal f) ->
+      find_instr (Ptrofs.unsigned ofs) f.(fn_code) = Some (Pbuiltin ef args res) ->
+      eval_builtin_args ge rs (rs SP) m args vargs ->
+      external_call ef ge vargs m t vres m' ->
+      rs' = nextinstr
+              (set_res res vres
+                (undef_regs (map preg_of (destroyed_by_builtin ef)) rs)) ->
+      step (State rs m) t (State rs' m')
+  | exec_step_external:
+      forall b ef args res rs m t rs' m',
+      rs PC = Vptr b Ptrofs.zero ->
+      Genv.find_funct_ptr ge b = Some (External ef) ->
+      external_call ef ge args m t res m' ->
+      extcall_arguments rs m (ef_sig ef) args ->
+      rs' = (set_pair (loc_external_result (ef_sig ef) ) res (undef_caller_save_regs rs)) #PC <- (rs RA) ->
+      step (State rs m) t (State rs' m').
+
 End RELSEM.
+
+(** Execution of whole programs. *)
+
+Inductive initial_state (p: program): state -> Prop :=
+  | initial_state_intro: forall m0,
+      let ge := Genv.globalenv p in
+      let rs0 :=
+        (Pregmap.init Vundef)
+        # PC <- (Genv.symbol_address ge p.(prog_main) Ptrofs.zero)
+        # SP <- Vnullptr
+        # RA <- Vnullptr in
+      Genv.init_mem p = Some m0 ->
+      initial_state p (State rs0 m0).
+
+Inductive final_state: state -> int -> Prop :=
+  | final_state_intro: forall rs m r,
+      rs PC = Vnullptr ->
+      rs R0 = Vint r ->
+      final_state (State rs m) r.
+
+Definition semantics (p: program) :=
+  Semantics step (initial_state p) final_state (Genv.globalenv p).
+
+(** Determinacy of the [Asm] semantics. *)
+
+Remark extcall_arguments_determ:
+  forall rs m sg args1 args2,
+  extcall_arguments rs m sg args1 -> extcall_arguments rs m sg args2 -> args1 = args2.
+Proof.
+  intros until m.
+  assert (A: forall l v1 v2,
+             extcall_arg rs m l v1 -> extcall_arg rs m l v2 -> v1 = v2).
+  { intros. inv H; inv H0; congruence. }
+  assert (B: forall p v1 v2,
+             extcall_arg_pair rs m p v1 -> extcall_arg_pair rs m p v2 -> v1 = v2).
+  { intros. inv H; inv H0.
+    eapply A; eauto.
+    f_equal; eapply A; eauto. }
+  assert (C: forall ll vl1, list_forall2 (extcall_arg_pair rs m) ll vl1 ->
+             forall vl2, list_forall2 (extcall_arg_pair rs m) ll vl2 -> vl1 = vl2).
+  {
+    induction 1; intros vl2 EA; inv EA.
+    auto.
+    f_equal; eauto. }
+  intros. eapply C; eauto.
+Qed.
+
+Lemma semantics_determinate: forall p, determinate (semantics p).
+Proof.
+Ltac Equalities :=
+  match goal with
+  | [ H1: ?a = ?b, H2: ?a = ?c |- _ ] =>
+      rewrite H1 in H2; inv H2; Equalities
+  | _ => idtac
+  end.
+  intros; constructor; simpl; intros.
+- (* determ *)
+  inv H; inv H0; Equalities.
+  split. constructor. auto.
+  discriminate.
+  discriminate.
+  assert (vargs0 = vargs) by (eapply eval_builtin_args_determ; eauto). subst vargs0.
+  exploit external_call_determ. eexact H5. eexact H11. intros [A B].
+  split. auto. intros. destruct B; auto. subst. auto.
+  assert (args0 = args) by (eapply extcall_arguments_determ; eauto). subst args0.
+  exploit external_call_determ. eexact H3. eexact H8. intros [A B].
+  split. auto. intros. destruct B; auto. subst. auto.
+- (* trace length *)
+  red; intros. inv H; simpl.
+  lia.
+  eapply external_call_trace_length; eauto.
+  eapply external_call_trace_length; eauto.
+- (* initial states *)
+  inv H; inv H0. f_equal. congruence.
+- (* final no step *)
+  assert (NOTNULL: forall b ofs, Vnullptr <> Vptr b ofs).
+  { intros; unfold Vnullptr; destruct Archi.ptr64; congruence. }
+  inv H. unfold Vzero in H0. red; intros; red; intros.
+  inv H; rewrite H0 in *; eelim NOTNULL; eauto.
+- (* final states *)
+  inv H; inv H0. congruence.
+Qed.
+
+(** Classification functions for processor registers (used in Asmgenproof). *)
+
+Definition data_preg (r: preg) : bool :=
+  match r with
+  | IR _ => true
+  | FR _ => true
+  | PC   => false
+  | RA   => false
+  end.
+
