ebpf/Asmgen.v
@@ -28,44 +28,69 @@ Local Open Scope error_monad_scope.
 
 (** Extracting integer registers. *)
 
-Definition preg_of (r: mreg) : res preg :=
-  match Asm.preg_of r with
-  | Some mr => OK mr
-  | _ => Error (msg "Floating numbers aren't available in eBPF")
+Definition ireg_of (r: mreg) : res ireg :=
+  match preg_of r with
+  | IR mr => OK mr
+  | FR mr => Error (msg "Floating numbers aren't available in eBPF")
+  | _ => Error (msg "Asmgen.ireg_of")
   end.
 
+Definition freg_of (r: mreg) : res freg :=
+  match preg_of r with
+  | FR mr => OK mr
+  | _ => Error (msg "Asmgen.freg_of")
+  end.
+
+(** Smart constructors for arithmetic operations. *)
+
+Definition addptrofs (rd rs: ireg) (n: ptrofs) (k: code) :=
+  if Ptrofs.eq_dec n Ptrofs.zero then
+    Palu MOV rd (inl rs) :: k
+  else
+    Palu MOV rd (inl rs) ::
+    Palu ADD rd (inr (Ptrofs.to_int n)) :: k.
 
 (** Translation of conditional branches. *)
 
-Definition transl_cbranch_sign (sign: Ctypes.signedness) (cmp: comparison) (r1: preg) (r2: preg+imm) (lbl: label) :=
+Definition transl_cbranch_signed (cmp: comparison) (r1: ireg) (r2: ireg+imm) (lbl: label) :=
   match cmp with
   | Ceq => Pjmpcmp EQ r1 r2 lbl
   | Cne => Pjmpcmp NE r1 r2 lbl
-  | Clt => Pjmpcmp (LT sign) r1 r2 lbl
-  | Cle => Pjmpcmp (LE sign) r1 r2 lbl
-  | Cgt => Pjmpcmp (GT sign) r1 r2 lbl
-  | Cge => Pjmpcmp (GE sign) r1 r2 lbl
+  | Clt => Pjmpcmp (LT Ctypes.Signed) r1 r2 lbl
+  | Cle => Pjmpcmp (LE Ctypes.Signed) r1 r2 lbl
+  | Cgt => Pjmpcmp (GT Ctypes.Signed) r1 r2 lbl
+  | Cge => Pjmpcmp (GE Ctypes.Signed) r1 r2 lbl
+  end.
+
+Definition transl_cbranch_unsigned (cmp: comparison) (r1: ireg) (r2: ireg+imm) (lbl: label) :=
+  match cmp with
+  | Ceq => Pjmpcmp EQ r1 r2 lbl
+  | Cne => Pjmpcmp NE r1 r2 lbl
+  | Clt => Pjmpcmp (LT Ctypes.Unsigned) r1 r2 lbl
+  | Cle => Pjmpcmp (LE Ctypes.Unsigned) r1 r2 lbl
+  | Cgt => Pjmpcmp (GT Ctypes.Unsigned) r1 r2 lbl
+  | Cge => Pjmpcmp (GE Ctypes.Unsigned) r1 r2 lbl
   end.
 
 Definition transl_cbranch (cond: condition) (args: list mreg) (lbl: label) (k: code) :=
   match cond, args with
   | Ccomp c, a1 :: a2 :: nil =>
-      do r1 <- preg_of a1;
-      do r2 <- preg_of a2;
-      OK (transl_cbranch_sign Ctypes.Signed c r1 (inl r2) lbl :: k)
+      do r1 <- ireg_of a1;
+      do r2 <- ireg_of a2;
+      OK (transl_cbranch_signed c r1 (inl r2) lbl :: k)
 
   | Ccompu c, a1 :: a2 :: nil =>
-      do r1 <- preg_of a1;
-      do r2 <- preg_of a2;
-      OK (transl_cbranch_sign Ctypes.Unsigned c r1 (inl r2) lbl :: k)
+      do r1 <- ireg_of a1;
+      do r2 <- ireg_of a2;
+      OK (transl_cbranch_unsigned c r1 (inl r2) lbl :: k)
 
   | Ccompimm c n, a1 :: nil =>
-      do r1 <- preg_of a1;
-      OK (transl_cbranch_sign Ctypes.Signed c r1 (inr n) lbl :: k)
+      do r1 <- ireg_of a1;
+      OK (transl_cbranch_signed c r1 (inr n) lbl :: k)
 
   | Ccompuimm c n, a1 :: nil =>
-      do r1 <- preg_of a1;
-      OK (transl_cbranch_sign Ctypes.Unsigned c r1 (inr n) lbl :: k)
+      do r1 <- ireg_of a1;
+      OK (transl_cbranch_unsigned c r1 (inr n) lbl :: k)
 
   | Ccompf _, _
   | Cnotcompf _, _
@@ -75,43 +100,56 @@ Definition transl_cbranch (cond: condition) (args: list mreg) (lbl: label) (k: c
   | _, _ => Error(msg "Asmgen.transl_cbranch")
   end.
 
-Definition transl_cond_sign (sign: Ctypes.signedness) (cmp: comparison) (r1: preg) (r2: preg+imm) :=
+Definition transl_cond_signed (cmp: comparison) (r1: ireg) (r2: ireg+imm) :=
   match cmp with
   | Ceq => Pcmp EQ r1 r2
   | Cne => Pcmp NE r1 r2
-  | Clt => Pcmp (LT sign) r1 r2
-  | Cle => Pcmp (LE sign) r1 r2
-  | Cgt => Pcmp (GT sign) r1 r2
-  | Cge => Pcmp (GE sign) r1 r2
+  | Clt => Pcmp (LT Ctypes.Signed) r1 r2
+  | Cle => Pcmp (LE Ctypes.Signed) r1 r2
+  | Cgt => Pcmp (GT Ctypes.Signed) r1 r2
+  | Cge => Pcmp (GE Ctypes.Signed) r1 r2
   end.
 
-Definition transl_cond_op (cond: condition) (rd: preg) (args: list mreg) (k: code) :=
+Definition transl_cond_unsigned (cmp: comparison) (r1: ireg) (r2: ireg+imm) :=
+  match cmp with
+  | Ceq => Pcmp EQ r1 r2
+  | Cne => Pcmp NE r1 r2
+  | Clt => Pcmp (LT Ctypes.Unsigned) r1 r2
+  | Cle => Pcmp (LE Ctypes.Unsigned) r1 r2
+  | Cgt => Pcmp (GT Ctypes.Unsigned) r1 r2
+  | Cge => Pcmp (GE Ctypes.Unsigned) r1 r2
+  end.
+
+Definition transl_cond_op (cond: condition) (r: mreg) (args: list mreg) (k: code) :=
   match cond, args with
   | Ccomp c, a1 :: a2 :: nil =>
-      do r1 <- preg_of a1;
-      do r2 <- preg_of a2;
-      OK (transl_cond_sign Ctypes.Signed c r1 (inl r2) :: k)
+      assertion (mreg_eq r a1);
+      do r1 <- ireg_of a1;
+      do r2 <- ireg_of a2;
+      OK (transl_cond_signed c r1 (inl r2) :: k)
 
   | Ccompu c, a1 :: a2 :: nil =>
-      do r1 <- preg_of a1;
-      do r2 <- preg_of a2;
-      OK (transl_cond_sign Ctypes.Unsigned c r1 (inl r2) :: k)
+      assertion (mreg_eq r a1);
+      do r1 <- ireg_of a1;
+      do r2 <- ireg_of a2;
+      OK (transl_cond_unsigned c r1 (inl r2) :: k)
 
   | Ccompimm c n, a1 :: nil =>
-      do r1 <- preg_of a1;
-      OK (transl_cond_sign Ctypes.Signed c r1 (inr n) :: k)
+      assertion (mreg_eq r a1);
+      do r1 <- ireg_of a1;
+      OK (transl_cond_signed c r1 (inr n) :: k)
 
   | Ccompuimm c n, a1 :: nil =>
-      do r1 <- preg_of a1;
-      OK (transl_cond_sign Ctypes.Unsigned c r1 (inr n) :: k)
+      assertion (mreg_eq r a1);
+      do r1 <- ireg_of a1;
+      OK (transl_cond_unsigned c r1 (inr n) :: k)
 
   | Ccompf c, _
   | Cnotcompf c, _
   | Ccompfs c, _
   | Cnotcompfs c, _ => Error (msg "Floating numbers aren't available in eBPF")
 
-  | _, _ =>
-      Error(msg "Asmgen.transl_cond_op")
+  | _, _ => Error (msg "Asmgen.transl_cond_op")
   end.
 
 (** Translation of the arithmetic operation [r <- op(args)].
@@ -120,155 +158,149 @@ Definition transl_cond_op (cond: condition) (rd: preg) (args: list mreg) (k: cod
 Definition transl_op (op: operation) (args: list mreg) (res: mreg) (k: code) :=
   match op, args with
   | Omove, a1 :: nil =>
-      do r <- preg_of res;
-      do r1 <- preg_of a1;
+      do r <- ireg_of res;
+      do r1 <- ireg_of a1;
       OK (Palu MOV r (inl r1) :: k)
 
   | Ointconst n, nil =>
-      do r <- preg_of res;
+      do r <- ireg_of res;
       OK (Palu MOV r (inr n) :: k)
 
   | Oaddrstack n, nil =>
-      do r <- preg_of res;
-
-      if Ptrofs.eq_dec n Ptrofs.zero then
-        OK (Palu MOV r (inl SP) :: k)
-      else
-        OK (Palu MOV r (inl SP) ::
-            Palu ADD r (inr (Int.repr (Ptrofs.signed n))) :: k)
+      do r <- ireg_of res;
+      OK (addptrofs r SP n k)
 
   | Oadd, a1 :: a2 :: nil =>
       assertion (mreg_eq a1 res);
-      do r <- preg_of res;
-      do r2 <- preg_of a2;
+      do r <- ireg_of res;
+      do r2 <- ireg_of a2;
       OK (Palu ADD r (inl r2) :: k)
 
   | Oaddimm n, a1 :: nil =>
       assertion (mreg_eq a1 res);
-      do r <- preg_of res;
+      do r <- ireg_of res;
       OK (Palu ADD r (inr n) :: k)
 
   | Oneg, a1 :: nil =>
       assertion (mreg_eq a1 res);
-      do r <- preg_of res;
+      do r <- ireg_of res;
       OK (Palu MUL r (inr (Int.repr (-1))) :: k)
 
   | Osub, a1 :: a2 :: nil =>
       assertion (mreg_eq a1 res);
-      do r <- preg_of res;
-      do r2 <- preg_of a2;
+      do r <- ireg_of res;
+      do r2 <- ireg_of a2;
       OK (Palu SUB r (inl r2) :: k)
 
   | Osubimm n, a1 :: nil =>
       assertion (mreg_eq a1 res);
-      do r <- preg_of res;
+      do r <- ireg_of res;
       OK (Palu SUB r (inr n) :: k)
 
   | Omul, a1 :: a2 :: nil =>
       assertion (mreg_eq a1 res);
-      do r <- preg_of res;
-      do r2 <- preg_of a2;
+      do r <- ireg_of res;
+      do r2 <- ireg_of a2;
       OK (Palu MUL r (inl r2) :: k)
 
   | Omulimm n, a1 :: nil =>
       assertion (mreg_eq a1 res);
-      do r <- preg_of res;
+      do r <- ireg_of res;
       OK (Palu MUL r (inr n) :: k)
 
   | Odivu, a1 :: a2 :: nil =>
       assertion (mreg_eq a1 res);
-      do r <- preg_of res;
-      do r2 <- preg_of a2;
+      do r <- ireg_of res;
+      do r2 <- ireg_of a2;
       OK (Palu DIV r (inl r2) :: k)
 
   | Odivuimm n, a1 :: nil =>
       assertion (mreg_eq a1 res);
-      do r <- preg_of res;
+      do r <- ireg_of res;
       OK (Palu DIV r (inr n) :: k)
 
   | Omodu, a1 :: a2 :: nil =>
       assertion (mreg_eq a1 res);
-      do r <- preg_of res;
-      do r2 <- preg_of a2;
+      do r <- ireg_of res;
+      do r2 <- ireg_of a2;
       OK (Palu MOD r (inl r2) :: k)
 
   | Omoduimm n, a1 :: nil =>
       assertion (mreg_eq a1 res);
-      do r <- preg_of res;
+      do r <- ireg_of res;
       OK (Palu MOD r (inr n) :: k)
 
   | Oand, a1 :: a2 :: nil =>
       assertion (mreg_eq a1 res);
-      do r <- preg_of res;
-      do r2 <- preg_of a2;
+      do r <- ireg_of res;
+      do r2 <- ireg_of a2;
       OK (Palu AND r (inl r2) :: k)
 
   | Oandimm n, a1 :: nil =>
       assertion (mreg_eq a1 res);
-      do r <- preg_of res;
+      do r <- ireg_of res;
       OK (Palu AND r (inr n) :: k)
 
   | Oor, a1 :: a2 :: nil =>
       assertion (mreg_eq a1 res);
-      do r <- preg_of res;
-      do r2 <- preg_of a2;
+      do r <- ireg_of res;
+      do r2 <- ireg_of a2;
       OK (Palu OR r (inl r2) :: k)
 
   | Oorimm n, a1 :: nil =>
       assertion (mreg_eq a1 res);
-      do r <- preg_of res;
+      do r <- ireg_of res;
       OK (Palu OR r (inr n) :: k)
 
   | Oxor, a1 :: a2 :: nil =>
       assertion (mreg_eq a1 res);
-      do r <- preg_of res;
-      do r2 <- preg_of a2;
+      do r <- ireg_of res;
+      do r2 <- ireg_of a2;
       OK (Palu XOR r (inl r2) :: k)
 
   | Oxorimm n, a1 :: nil =>
       assertion (mreg_eq a1 res);
-      do r <- preg_of res;
+      do r <- ireg_of res;
       OK (Palu XOR r (inr n) :: k)
 
   | Oshl, a1 :: a2 :: nil =>
       assertion (mreg_eq a1 res);
-      do r <- preg_of res;
-      do r2 <- preg_of a2;
+      do r <- ireg_of res;
+      do r2 <- ireg_of a2;
       OK (Palu LSH r (inl r2) :: k)
 
   | Oshlimm n, a1 :: nil =>
       assertion (mreg_eq a1 res);
-      do r <- preg_of res;
+      do r <- ireg_of res;
       OK (Palu LSH r (inr n) :: k)
 
   | Oshr, a1 :: a2 :: nil =>
       assertion (mreg_eq a1 res);
-      do r <- preg_of res;
-      do r2 <- preg_of a2;
-      OK (Palu RSH r (inl r2) :: k)
+      do r <- ireg_of res;
+      do r2 <- ireg_of a2;
+      OK (Palu ARSH r (inl r2) :: k)
 
   | Oshrimm n, a1 :: nil =>
       assertion (mreg_eq a1 res);
-      do r <- preg_of res;
-      OK (Palu RSH r (inr n) :: k)
+      do r <- ireg_of res;
+      OK (Palu ARSH r (inr n) :: k)
 
   | Oshru, a1 :: a2 :: nil =>
       assertion (mreg_eq a1 res);
-      do r <- preg_of res;
-      do r2 <- preg_of a2;
-      OK (Palu ARSH r (inl r2) :: k)
+      do r <- ireg_of res;
+      do r2 <- ireg_of a2;
+      OK (Palu RSH r (inl r2) :: k)
 
   | Oshruimm n, a1 :: nil =>
       assertion (mreg_eq a1 res);
-      do r <- preg_of res;
-      OK (Palu ARSH r (inr n) :: k)
+      do r <- ireg_of res;
+      OK (Palu RSH r (inr n) :: k)
 
   | Ocmp cmp, _ =>
-      do r <- preg_of res;
-      transl_cond_op cmp r args k
+      transl_cond_op cmp res args k
 
   (*c Following operations aren't available in eBPF, and will throw errors in this step *)
-  | Oaddrsymbol s ofs, nil => Error (msg "global variables are not available in eBPF")
+  | Oaddrsymbol s ofs, nil => Error (msg "Global variables are not yet available in eBPF")
 
   | Ocast8signed, a1 :: nil => Error (msg "cast8signed is not available in eBPF")
   | Ocast16signed, a1 :: nil => Error (msg "cast16signed is not available in eBPF")
@@ -327,11 +359,12 @@ Definition transl_op (op: operation) (args: list mreg) (res: mreg) (k: code) :=
 
 Definition transl_typ (typ: typ): res (sizeOp) :=
   match typ with
-  | Tint | Tany32 => OK Word
+  | Tany32 => OK Word
+  | Tint => OK SignedWord
 
   | Tsingle | Tfloat => Error (msg "Floating numbers aren't available in eBPF")
 
-  | _ => Error (msg "Asmgen.transl_memory_access")
+  | _ => Error (msg "Asmgen.transl_typ")
   end.
 
 
@@ -343,45 +376,61 @@ Definition transl_memory_access (chunk: memory_chunk): res (sizeOp) :=
 
   | Mint16unsigned => OK HalfWord
 
-  | Mint32 | Many32 => OK Word
+  | Many32 => OK Word
+
+  | Mint32 => OK SignedWord
 
   | Mfloat32 | Mfloat64 => Error (msg "Floating numbers aren't available in eBPF")
 
   | _ => Error (msg "Asmgen.transl_memory_access")
   end.
 
+Definition stack_load (ofs: ptrofs) (ty: typ) (dst: mreg) (k: code): res (list instruction) :=
+  do r <- ireg_of dst;
+  do size <- transl_typ ty;
+  OK (Pload size r SP ofs :: k).
+
+Definition stack_store (ofs: ptrofs) (ty: typ) (src: mreg) (k: code): res (list instruction) :=
+  do r <- ireg_of src;
+  do size <- transl_typ ty;
+  OK (Pstore size SP (inl r) ofs :: k).
+
 Definition transl_load (chunk: memory_chunk) (addr: addressing)
            (args: list mreg) (dst: mreg) (k: code): res (list instruction) :=
   match addr, args with
   | Aindexed ofs, a1 :: nil =>
-      do r <- preg_of dst;
-      do r1 <- preg_of a1;
+      do r <- ireg_of dst;
+      do r1 <- ireg_of a1;
       do size <- transl_memory_access chunk;
       OK (Pload size r r1 ofs :: k)
 
   | Ainstack ofs, nil =>
-      do r <- preg_of dst;
+      do r <- ireg_of dst;
       do size <- transl_memory_access chunk;
       OK (Pload size r SP ofs :: k)
 
-  | _, _ => Error(msg "transl_load.Mint32")
+  | Aglobal _ _, _ => Error(msg "Global variables are not yet available in eBPF")
+
+  | _, _ => Error(msg "Asmgen.transl_load")
   end.
 
 Definition transl_store (chunk: memory_chunk) (addr: addressing)
            (args: list mreg) (src: mreg) (k: code): res (list instruction) :=
   match addr, args with
   | Aindexed ofs, a1 :: nil =>
-      do r <- preg_of src;
-      do r1 <- preg_of a1;
+      do r <- ireg_of src;
+      do r1 <- ireg_of a1;
       do size <- transl_memory_access chunk;
-      OK (Pstore size r (inl r1) ofs :: k)
+      OK (Pstore size r1 (inl r) ofs :: k)
 
   | Ainstack ofs, nil =>
-      do r <- preg_of src;
+      do r <- ireg_of src;
       do size <- transl_memory_access chunk;
-      OK (Pstore size r (inl SP) ofs :: k)
+      OK (Pstore size SP (inl r) ofs :: k)
 
-  | _, _ => Error(msg "transl_store.Mint32")
+  | Aglobal _ _, _ => Error(msg "Global variables are not yet available in eBPF")
+
+  | _, _ => Error(msg "Asmgen.transl_store")
   end.
 
 (** Translation of a Mach instruction. *)
@@ -389,15 +438,9 @@ Definition transl_store (chunk: memory_chunk) (addr: addressing)
 Definition transl_instr (f: Mach.function) (i: Mach.instruction)
                         (ep: bool) (k: code): res (list instruction) :=
   match i with
-  | Mgetstack ofs ty dst =>
-      do r <- preg_of dst;
-      do size <- transl_typ ty;
-      OK (Pload size r SP ofs :: k)
+  | Mgetstack ofs ty dst => stack_load ofs ty dst k
 
-  | Msetstack src ofs ty =>
-      do r <- preg_of src;
-      do size <- transl_typ ty;
-      OK (Pstore size r (inl SP) ofs :: k)
+  | Msetstack src ofs ty => stack_store ofs ty src k
 
   | Mgetparam _ _ _ => Error (msg "Functions with more than 5 arguments aren't available in eBPF")
 
@@ -410,7 +453,7 @@ Definition transl_instr (f: Mach.function) (i: Mach.instruction)
   | Mcall sig (inr symb) => OK (Pcall symb sig :: k)
 
   | Mtailcall sig (inr symb) =>
-      OK (Pfreeframe f.(fn_stacksize) f.(fn_link_ofs) :: Pjmp (inr symb) :: k)
+      OK (Pfreeframe f.(fn_stacksize) f.(fn_retaddr_ofs) f.(fn_link_ofs) :: Pjmp (inr symb) :: k)
 
   | Mcall sig (inl r)
   | Mtailcall sig (inl r) => Error (msg "Call from function pointer aren't available in eBPF")
@@ -423,20 +466,16 @@ Definition transl_instr (f: Mach.function) (i: Mach.instruction)
 
   | Mcond cond args lbl => transl_cbranch cond args lbl k
 
-  | Mjumptable arg tbl => Error (msg "Mjumptable")
-  (*     do r <- ireg_of arg; *)
-  (*     OK (Pbtbl r tbl :: k) *)
+  | Mjumptable arg tbl => Error (msg "Internal error: Jumptable have been generated, but aren't available in eBPF")
 
-  | Mreturn => OK (Pfreeframe f.(fn_stacksize) f.(fn_link_ofs) :: Pret :: k)
+  | Mreturn => OK (Pfreeframe f.(fn_stacksize) f.(fn_retaddr_ofs) f.(fn_link_ofs) :: Pret :: k)
   end.
 
 (** Translation of a code sequence *)
 
 Definition it1_is_parent (before: bool) (i: Mach.instruction) : bool :=
   match i with
-  | Msetstack src ofs ty => before
-  | Mgetparam ofs ty dst => negb (mreg_eq dst I0)
-  | Mop op args res => before && negb (mreg_eq res I0)
+  | Msetstack _ _ _
   | _ => false
   end.
 
@@ -474,7 +513,7 @@ Definition transl_code' (f: Mach.function) (il: list Mach.instruction) (it1p: bo
 Definition transl_function (f: Mach.function) :=
   do c <- transl_code' f f.(Mach.fn_code) true;
   OK (mkfunction f.(Mach.fn_sig)
-    (Pallocframe f.(fn_stacksize) f.(fn_link_ofs) :: c)).
+    (Pallocframe f.(fn_stacksize) f.(fn_retaddr_ofs) f.(fn_link_ofs) :: c)).
 
 Definition transf_function (f: Mach.function) : res Asm.function :=
   do tf <- transl_function f;
