ebpf/ConstpropOpproof.v
@@ -1,0 +1,529 @@
+(* *********************************************************************)
+(*                                                                     *)
+(*              The Compcert verified compiler                         *)
+(*                                                                     *)
+(*                 Xavier Leroy, INRIA Paris                           *)
+(*                                                                     *)
+(*  Copyright Institut National de Recherche en Informatique et en     *)
+(*  Automatique.  All rights reserved.  This file is distributed       *)
+(*  under the terms of the INRIA Non-Commercial License Agreement.     *)
+(*                                                                     *)
+(* *********************************************************************)
+
+(** Correctness proof for operator strength reduction. *)
+
+Require Import Coqlib Compopts.
+Require Import Integers Floats Values Memory Globalenvs Events.
+Require Import Op Registers RTL ValueDomain.
+Require Import ConstpropOp.
+
+Section STRENGTH_REDUCTION.
+
+Variable bc: block_classification.
+Variable ge: genv.
+Hypothesis GENV: genv_match bc ge.
+Variable sp: block.
+Hypothesis STACK: bc sp = BCstack.
+Variable ae: AE.t.
+Variable e: regset.
+Variable m: mem.
+Hypothesis MATCH: ematch bc e ae.
+
+Lemma match_G:
+  forall r id ofs,
+  AE.get r ae = Ptr(Gl id ofs) -> Val.lessdef e#r (Genv.symbol_address ge id ofs).
+Proof.
+  intros. apply vmatch_ptr_gl with bc; auto. rewrite <- H. apply MATCH.
+Qed.
+
+Lemma match_S:
+  forall r ofs,
+  AE.get r ae = Ptr(Stk ofs) -> Val.lessdef e#r (Vptr sp ofs).
+Proof.
+  intros. apply vmatch_ptr_stk with bc; auto. rewrite <- H. apply MATCH.
+Qed.
+
+Ltac InvApproxRegs :=
+  match goal with
+  | [ H: _ :: _ = _ :: _ |- _ ] =>
+        injection H; clear H; intros; InvApproxRegs
+  | [ H: ?v = AE.get ?r ae |- _ ] =>
+        generalize (MATCH r); rewrite <- H; clear H; intro; InvApproxRegs
+  | _ => idtac
+  end.
+
+Ltac SimplVM :=
+  match goal with
+  | [ H: vmatch _ ?v (I ?n) |- _ ] =>
+      let E := fresh in
+      assert (E: v = Vint n) by (inversion H; auto);
+      rewrite E in *; clear H; SimplVM
+  | [ H: vmatch _ ?v (L ?n) |- _ ] =>
+      let E := fresh in
+      assert (E: v = Vlong n) by (inversion H; auto);
+      rewrite E in *; clear H; SimplVM
+  | [ H: vmatch _ ?v (F ?n) |- _ ] =>
+      let E := fresh in
+      assert (E: v = Vfloat n) by (inversion H; auto);
+      rewrite E in *; clear H; SimplVM
+  | [ H: vmatch _ ?v (FS ?n) |- _ ] =>
+      let E := fresh in
+      assert (E: v = Vsingle n) by (inversion H; auto);
+      rewrite E in *; clear H; SimplVM
+  | [ H: vmatch _ ?v (Ptr(Gl ?id ?ofs)) |- _ ] =>
+      let E := fresh in
+      assert (E: Val.lessdef v (Genv.symbol_address ge id ofs)) by (eapply vmatch_ptr_gl; eauto);
+      clear H; SimplVM
+  | [ H: vmatch _ ?v (Ptr(Stk ?ofs)) |- _ ] =>
+      let E := fresh in
+      assert (E: Val.lessdef v (Vptr sp ofs)) by (eapply vmatch_ptr_stk; eauto);
+      clear H; SimplVM
+  | _ => idtac
+  end.
+
+Lemma const_for_result_correct:
+  forall a op v,
+  const_for_result a = Some op ->
+  vmatch bc v a ->
+  exists v', eval_operation ge (Vptr sp Ptrofs.zero) op nil m = Some v' /\ Val.lessdef v v'.
+Proof.
+  unfold const_for_result. generalize Archi.ptr64; intros ptr64; intros.
+  destruct a; inv H; SimplVM.
+- (* integer *)
+  exists (Vint n); auto.
+- (* float *)
+  destruct (Compopts.generate_float_constants tt); inv H2. exists (Vfloat f); auto.
+- (* single *)
+  destruct (Compopts.generate_float_constants tt); inv H2. exists (Vsingle f); auto.
+- (* pointer *)
+  destruct p; try discriminate; SimplVM.
+  + (* global *)
+    inv H2. exists (Genv.symbol_address ge id ofs); auto.
+  + (* stack *)
+    inv H2. exists (Vptr sp ofs); split; auto. simpl. rewrite Ptrofs.add_zero_l; auto.
+Qed.
+
+Lemma cond_strength_reduction_correct:
+  forall cond args vl,
+  vl = map (fun r => AE.get r ae) args ->
+  let (cond', args') := cond_strength_reduction cond args vl in
+  eval_condition cond' e##args' m = eval_condition cond e##args m.
+Proof.
+  intros until vl. unfold cond_strength_reduction.
+  case (cond_strength_reduction_match cond args vl); simpl; intros; InvApproxRegs; SimplVM.
+- apply Val.swap_cmp_bool.
+- auto.
+- apply Val.swap_cmpu_bool.
+- auto.
+- auto.
+Qed.
+
+Lemma make_cmp_base_correct:
+  forall c args vl,
+  vl = map (fun r => AE.get r ae) args ->
+  let (op', args') := make_cmp_base c args vl in
+  exists v, eval_operation ge (Vptr sp Ptrofs.zero) op' e##args' m = Some v
+         /\ Val.lessdef (Val.of_optbool (eval_condition c e##args m)) v.
+Proof.
+  intros. unfold make_cmp_base.
+  generalize (cond_strength_reduction_correct c args vl H).
+  destruct (cond_strength_reduction c args vl) as [c' args']. intros EQ.
+  econstructor; split. simpl; eauto. rewrite EQ. auto.
+Qed.
+
+Lemma make_cmp_correct:
+  forall c args vl,
+  vl = map (fun r => AE.get r ae) args ->
+  let (op', args') := make_cmp c args vl in
+  exists v, eval_operation ge (Vptr sp Ptrofs.zero) op' e##args' m = Some v
+         /\ Val.lessdef (Val.of_optbool (eval_condition c e##args m)) v.
+Proof.
+  intros c args vl.
+  assert (Y: forall r, vincl (AE.get r ae) (Uns Ptop 1) = true ->
+             e#r = Vundef \/ e#r = Vint Int.zero \/ e#r = Vint Int.one).
+  { intros. apply vmatch_Uns_1 with bc Ptop. eapply vmatch_ge. eapply vincl_ge; eauto. apply MATCH. }
+  unfold make_cmp. case (make_cmp_match c args vl); intros.
+- unfold make_cmp_imm_eq.
+  destruct (Int.eq_dec n Int.one && vincl v1 (Uns Ptop 1)) eqn:E1.
++ simpl in H; inv H. InvBooleans. subst n.
+  exists (e#r1); split; auto. simpl.
+  exploit Y; eauto. intros [A | [A | A]]; rewrite A; simpl; auto.
++ destruct (Int.eq_dec n Int.zero && vincl v1 (Uns Ptop 1)) eqn:E0.
+* simpl in H; inv H. InvBooleans. subst n.
+  exists (Val.xor e#r1 (Vint Int.one)); split; auto. simpl.
+  exploit Y; eauto. intros [A | [A | A]]; rewrite A; simpl; auto.
+* apply make_cmp_base_correct; auto.
+- unfold make_cmp_imm_ne.
+  destruct (Int.eq_dec n Int.zero && vincl v1 (Uns Ptop 1)) eqn:E0.
++ simpl in H; inv H. InvBooleans. subst n.
+  exists (e#r1); split; auto. simpl.
+  exploit Y; eauto. intros [A | [A | A]]; rewrite A; simpl; auto.
++ destruct (Int.eq_dec n Int.one && vincl v1 (Uns Ptop 1)) eqn:E1.
+* simpl in H; inv H. InvBooleans. subst n.
+  exists (Val.xor e#r1 (Vint Int.one)); split; auto. simpl.
+  exploit Y; eauto. intros [A | [A | A]]; rewrite A; simpl; auto.
+* apply make_cmp_base_correct; auto.
+- unfold make_cmp_imm_eq.
+  destruct (Int.eq_dec n Int.one && vincl v1 (Uns Ptop 1)) eqn:E1.
++ simpl in H; inv H. InvBooleans. subst n.
+  exists (e#r1); split; auto. simpl.
+  exploit Y; eauto. intros [A | [A | A]]; rewrite A; simpl; auto.
++ destruct (Int.eq_dec n Int.zero && vincl v1 (Uns Ptop 1)) eqn:E0.
+* simpl in H; inv H. InvBooleans. subst n.
+  exists (Val.xor e#r1 (Vint Int.one)); split; auto. simpl.
+  exploit Y; eauto. intros [A | [A | A]]; rewrite A; simpl; auto.
+* apply make_cmp_base_correct; auto.
+- unfold make_cmp_imm_ne.
+  destruct (Int.eq_dec n Int.zero && vincl v1 (Uns Ptop 1)) eqn:E0.
++ simpl in H; inv H. InvBooleans. subst n.
+  exists (e#r1); split; auto. simpl.
+  exploit Y; eauto. intros [A | [A | A]]; rewrite A; simpl; auto.
++ destruct (Int.eq_dec n Int.one && vincl v1 (Uns Ptop 1)) eqn:E1.
+* simpl in H; inv H. InvBooleans. subst n.
+  exists (Val.xor e#r1 (Vint Int.one)); split; auto. simpl.
+  exploit Y; eauto. intros [A | [A | A]]; rewrite A; simpl; auto.
+* apply make_cmp_base_correct; auto.
+- apply make_cmp_base_correct; auto.
+Qed.
+
+Lemma make_addimm_correct:
+  forall n r,
+  let (op, args) := make_addimm n r in
+  exists v, eval_operation ge (Vptr sp Ptrofs.zero) op e##args m = Some v /\ Val.lessdef (Val.add e#r (Vint n)) v.
+Proof.
+  intros. unfold make_addimm.
+  predSpec Int.eq Int.eq_spec n Int.zero; intros.
+  subst. exists (e#r); split; auto.
+  destruct (e#r); simpl; auto; rewrite ?Int.add_zero, ?Ptrofs.add_zero; auto.
+  exists (Val.add e#r (Vint n)); split; auto.
+Qed.
+
+Lemma make_shlimm_correct:
+  forall n r1 r2,
+  e#r2 = Vint n ->
+  let (op, args) := make_shlimm n r1 r2 in
+  exists v, eval_operation ge (Vptr sp Ptrofs.zero) op e##args m = Some v /\ Val.lessdef (Val.shl e#r1 (Vint n)) v.
+Proof.
+  intros; unfold make_shlimm.
+  predSpec Int.eq Int.eq_spec n Int.zero; intros. subst.
+  exists (e#r1); split; auto. destruct (e#r1); simpl; auto. rewrite Int.shl_zero. auto.
+  destruct (Int.ltu n Int.iwordsize).
+  econstructor; split. simpl. eauto. auto.
+  econstructor; split. simpl. eauto. rewrite H; auto.
+Qed.
+
+Lemma make_shrimm_correct:
+  forall n r1 r2,
+  e#r2 = Vint n ->
+  let (op, args) := make_shrimm n r1 r2 in
+  exists v, eval_operation ge (Vptr sp Ptrofs.zero) op e##args m = Some v /\ Val.lessdef (Val.shr e#r1 (Vint n)) v.
+Proof.
+  intros; unfold make_shrimm.
+  predSpec Int.eq Int.eq_spec n Int.zero; intros. subst.
+  exists (e#r1); split; auto. destruct (e#r1); simpl; auto. rewrite Int.shr_zero. auto.
+  destruct (Int.ltu n Int.iwordsize).
+  econstructor; split. simpl. eauto. auto.
+  econstructor; split. simpl. eauto. rewrite H; auto.
+Qed.
+
+Lemma make_shruimm_correct:
+  forall n r1 r2,
+  e#r2 = Vint n ->
+  let (op, args) := make_shruimm n r1 r2 in
+  exists v, eval_operation ge (Vptr sp Ptrofs.zero) op e##args m = Some v /\ Val.lessdef (Val.shru e#r1 (Vint n)) v.
+Proof.
+  intros; unfold make_shruimm.
+  predSpec Int.eq Int.eq_spec n Int.zero; intros. subst.
+  exists (e#r1); split; auto. destruct (e#r1); simpl; auto. rewrite Int.shru_zero. auto.
+  destruct (Int.ltu n Int.iwordsize).
+  econstructor; split. simpl. eauto. auto.
+  econstructor; split. simpl. eauto. rewrite H; auto.
+Qed.
+
+Lemma make_mulimm_correct:
+  forall n r1 r2,
+  e#r2 = Vint n ->
+  let (op, args) := make_mulimm n r1 r2 in
+  exists v, eval_operation ge (Vptr sp Ptrofs.zero) op e##args m = Some v /\ Val.lessdef (Val.mul e#r1 (Vint n)) v.
+Proof.
+  intros; unfold make_mulimm.
+  predSpec Int.eq Int.eq_spec n Int.zero; intros. subst.
+  exists (Vint Int.zero); split; auto. destruct (e#r1); simpl; auto. rewrite Int.mul_zero; auto.
+  predSpec Int.eq Int.eq_spec n Int.one; intros. subst.
+  exists (e#r1); split; auto. destruct (e#r1); simpl; auto. rewrite Int.mul_one; auto.
+  destruct (Int.is_power2 n) eqn:?; intros.
+  rewrite (Val.mul_pow2 e#r1 _ _ Heqo). econstructor; split. simpl; eauto. auto.
+  econstructor; split; eauto. simpl. rewrite H; auto.
+Qed.
+
+Lemma make_divimm_correct:
+  forall n r1 r2 v,
+  Val.divs e#r1 e#r2 = Some v ->
+  e#r2 = Vint n ->
+  let (op, args) := make_divimm n r1 r2 in
+  exists w, eval_operation ge (Vptr sp Ptrofs.zero) op e##args m = Some w /\ Val.lessdef v w.
+Proof.
+  intros; unfold make_divimm.
+  predSpec Int.eq Int.eq_spec n Int.one; intros. subst. rewrite H0 in H.
+  destruct (e#r1) eqn:?;
+    try (rewrite Val.divs_one in H; exists (Vint i); split; simpl; try rewrite Heqv0; auto);
+    inv H; auto.
+  destruct (Int.is_power2 n) eqn:?.
+  destruct (Int.ltu i (Int.repr 31)) eqn:?.
+  exists v; split; auto. simpl. eapply Val.divs_pow2; eauto. congruence.
+  exists v; auto.
+  exists v; auto.
+Qed.
+
+Lemma make_divuimm_correct:
+  forall n r1 r2 v,
+  Val.divu e#r1 e#r2 = Some v ->
+  e#r2 = Vint n ->
+  let (op, args) := make_divuimm n r1 r2 in
+  exists w, eval_operation ge (Vptr sp Ptrofs.zero) op e##args m = Some w /\ Val.lessdef v w.
+Proof.
+  intros; unfold make_divuimm.
+  predSpec Int.eq Int.eq_spec n Int.one; intros. subst. rewrite H0 in H.
+  destruct (e#r1) eqn:?;
+    try (rewrite Val.divu_one in H; exists (Vint i); split; simpl; try rewrite Heqv0; auto);
+    inv H; auto.
+  destruct (Int.is_power2 n) eqn:?.
+  econstructor; split. simpl; eauto.
+  rewrite H0 in H. erewrite Val.divu_pow2 by eauto. auto.
+  exists v; auto.
+Qed.
+
+Lemma make_moduimm_correct:
+  forall n r1 r2 v,
+  Val.modu e#r1 e#r2 = Some v ->
+  e#r2 = Vint n ->
+  let (op, args) := make_moduimm n r1 r2 in
+  exists w, eval_operation ge (Vptr sp Ptrofs.zero) op e##args m = Some w /\ Val.lessdef v w.
+Proof.
+  intros; unfold make_moduimm.
+  destruct (Int.is_power2 n) eqn:?.
+  exists v; split; auto. simpl. decEq. eapply Val.modu_pow2; eauto. congruence.
+  exists v; auto.
+Qed.
+
+Lemma make_andimm_correct:
+  forall n r x,
+  vmatch bc e#r x ->
+  let (op, args) := make_andimm n r x in
+  exists v, eval_operation ge (Vptr sp Ptrofs.zero) op e##args m = Some v /\ Val.lessdef (Val.and e#r (Vint n)) v.
+Proof.
+  intros; unfold make_andimm.
+  predSpec Int.eq Int.eq_spec n Int.zero; intros.
+  subst n. exists (Vint Int.zero); split; auto. destruct (e#r); simpl; auto. rewrite Int.and_zero; auto.
+  predSpec Int.eq Int.eq_spec n Int.mone; intros.
+  subst n. exists (e#r); split; auto. destruct (e#r); simpl; auto. rewrite Int.and_mone; auto.
+  destruct (match x with Uns _ k => Int.eq (Int.zero_ext k (Int.not n)) Int.zero
+                       | _ => false end) eqn:UNS.
+  destruct x; try congruence.
+  exists (e#r); split; auto.
+  inv H; auto. simpl. replace (Int.and i n) with i; auto.
+  generalize (Int.eq_spec (Int.zero_ext n0 (Int.not n)) Int.zero); rewrite UNS; intro EQ.
+  Int.bit_solve. destruct (zlt i0 n0).
+  replace (Int.testbit n i0) with (negb (Int.testbit Int.zero i0)).
+  rewrite Int.bits_zero. simpl. rewrite andb_true_r. auto.
+  rewrite <- EQ. rewrite Int.bits_zero_ext by lia. rewrite zlt_true by auto.
+  rewrite Int.bits_not by auto. apply negb_involutive.
+  rewrite H6 by auto. auto.
+  econstructor; split; eauto. auto.
+Qed.
+
+Lemma make_orimm_correct:
+  forall n r,
+  let (op, args) := make_orimm n r in
+  exists v, eval_operation ge (Vptr sp Ptrofs.zero) op e##args m = Some v /\ Val.lessdef (Val.or e#r (Vint n)) v.
+Proof.
+  intros; unfold make_orimm.
+  predSpec Int.eq Int.eq_spec n Int.zero; intros.
+  subst n. exists (e#r); split; auto. destruct (e#r); simpl; auto. rewrite Int.or_zero; auto.
+  predSpec Int.eq Int.eq_spec n Int.mone; intros.
+  subst n. exists (Vint Int.mone); split; auto. destruct (e#r); simpl; auto. rewrite Int.or_mone; auto.
+  econstructor; split; eauto. auto.
+Qed.
+
+Lemma make_xorimm_correct:
+  forall n r,
+  let (op, args) := make_xorimm n r in
+  exists v, eval_operation ge (Vptr sp Ptrofs.zero) op e##args m = Some v /\ Val.lessdef (Val.xor e#r (Vint n)) v.
+Proof.
+  intros; unfold make_xorimm.
+  predSpec Int.eq Int.eq_spec n Int.zero; intros.
+  subst n. exists (e#r); split; auto. destruct (e#r); simpl; auto. rewrite Int.xor_zero; auto.
+  predSpec Int.eq Int.eq_spec n Int.mone; intros.
+  subst n. exists (Val.notint e#r); split; auto.
+  econstructor; split; eauto. auto.
+Qed.
+
+Lemma make_mulfimm_correct:
+  forall n r1 r2,
+  e#r2 = Vfloat n ->
+  let (op, args) := make_mulfimm n r1 r1 r2 in
+  exists v, eval_operation ge (Vptr sp Ptrofs.zero) op e##args m = Some v /\ Val.lessdef (Val.mulf e#r1 e#r2) v.
+Proof.
+  intros; unfold make_mulfimm.
+  destruct (Float.eq_dec n (Float.of_int (Int.repr 2))); intros.
+  simpl. econstructor; split. eauto. rewrite H; subst n.
+  destruct (e#r1); simpl; auto. rewrite Float.mul2_add; auto.
+  simpl. econstructor; split; eauto.
+Qed.
+
+Lemma make_mulfimm_correct_2:
+  forall n r1 r2,
+  e#r1 = Vfloat n ->
+  let (op, args) := make_mulfimm n r2 r1 r2 in
+  exists v, eval_operation ge (Vptr sp Ptrofs.zero) op e##args m = Some v /\ Val.lessdef (Val.mulf e#r1 e#r2) v.
+Proof.
+  intros; unfold make_mulfimm.
+  destruct (Float.eq_dec n (Float.of_int (Int.repr 2))); intros.
+  simpl. econstructor; split. eauto. rewrite H; subst n.
+  destruct (e#r2); simpl; auto. rewrite Float.mul2_add; auto.
+  rewrite Float.mul_commut; auto.
+  simpl. econstructor; split; eauto.
+Qed.
+
+Lemma make_mulfsimm_correct:
+  forall n r1 r2,
+  e#r2 = Vsingle n ->
+  let (op, args) := make_mulfsimm n r1 r1 r2 in
+  exists v, eval_operation ge (Vptr sp Ptrofs.zero) op e##args m = Some v /\ Val.lessdef (Val.mulfs e#r1 e#r2) v.
+Proof.
+  intros; unfold make_mulfsimm.
+  destruct (Float32.eq_dec n (Float32.of_int (Int.repr 2))); intros.
+  simpl. econstructor; split. eauto. rewrite H; subst n.
+  destruct (e#r1); simpl; auto. rewrite Float32.mul2_add; auto.
+  simpl. econstructor; split; eauto.
+Qed.
+
+Lemma make_mulfsimm_correct_2:
+  forall n r1 r2,
+  e#r1 = Vsingle n ->
+  let (op, args) := make_mulfsimm n r2 r1 r2 in
+  exists v, eval_operation ge (Vptr sp Ptrofs.zero) op e##args m = Some v /\ Val.lessdef (Val.mulfs e#r1 e#r2) v.
+Proof.
+  intros; unfold make_mulfsimm.
+  destruct (Float32.eq_dec n (Float32.of_int (Int.repr 2))); intros.
+  simpl. econstructor; split. eauto. rewrite H; subst n.
+  destruct (e#r2); simpl; auto. rewrite Float32.mul2_add; auto.
+  rewrite Float32.mul_commut; auto.
+  simpl. econstructor; split; eauto.
+Qed.
+
+Lemma make_cast8signed_correct:
+  forall r x,
+  vmatch bc e#r x ->
+  let (op, args) := make_cast8signed r x in
+  exists v, eval_operation ge (Vptr sp Ptrofs.zero) op e##args m = Some v /\ Val.lessdef (Val.sign_ext 8 e#r) v.
+Proof.
+  intros; unfold make_cast8signed. destruct (vincl x (Sgn Ptop 8)) eqn:INCL.
+  exists e#r; split; auto.
+  assert (V: vmatch bc e#r (Sgn Ptop 8)).
+  { eapply vmatch_ge; eauto. apply vincl_ge; auto. }
+  inv V; simpl; auto. rewrite is_sgn_sign_ext in H4 by auto. rewrite H4; auto.
+  econstructor; split; simpl; eauto.
+Qed.
+
+Lemma make_cast16signed_correct:
+  forall r x,
+  vmatch bc e#r x ->
+  let (op, args) := make_cast16signed r x in
+  exists v, eval_operation ge (Vptr sp Ptrofs.zero) op e##args m = Some v /\ Val.lessdef (Val.sign_ext 16 e#r) v.
+Proof.
+  intros; unfold make_cast16signed. destruct (vincl x (Sgn Ptop 16)) eqn:INCL.
+  exists e#r; split; auto.
+  assert (V: vmatch bc e#r (Sgn Ptop 16)).
+  { eapply vmatch_ge; eauto. apply vincl_ge; auto. }
+  inv V; simpl; auto. rewrite is_sgn_sign_ext in H4 by auto. rewrite H4; auto.
+  econstructor; split; simpl; eauto.
+Qed.
+
+Lemma op_strength_reduction_correct:
+  forall op args vl v,
+  vl = map (fun r => AE.get r ae) args ->
+  eval_operation ge (Vptr sp Ptrofs.zero) op e##args m = Some v ->
+  let (op', args') := op_strength_reduction op args vl in
+  exists w, eval_operation ge (Vptr sp Ptrofs.zero) op' e##args' m = Some w /\ Val.lessdef v w.
+Proof.
+  intros until v; unfold op_strength_reduction;
+  case (op_strength_reduction_match op args vl); simpl; intros.
+- (* cast8signed *)
+  InvApproxRegs; SimplVM; inv H0. apply make_cast8signed_correct; auto.
+- (* cast16signed *)
+  InvApproxRegs; SimplVM; inv H0. apply make_cast16signed_correct; auto.
+- (* add 1 *)
+  rewrite Val.add_commut in H0. InvApproxRegs; SimplVM; inv H0. apply make_addimm_correct; auto.
+- (* add 2 *)
+  InvApproxRegs; SimplVM; inv H0. apply make_addimm_correct; auto.
+- (* sub *)
+  InvApproxRegs; SimplVM; inv H0. rewrite Val.sub_add_opp. apply make_addimm_correct; auto.
+- (* mul 1 *)
+  rewrite Val.mul_commut in H0. InvApproxRegs; SimplVM; inv H0. apply make_mulimm_correct; auto.
+- (* mul 2*)
+  InvApproxRegs; SimplVM; inv H0. apply make_mulimm_correct; auto.
+- (* divs *)
+  assert (e#r2 = Vint n2). clear H0. InvApproxRegs; SimplVM; auto.
+  apply make_divimm_correct; auto.
+- (* divu *)
+  assert (e#r2 = Vint n2). clear H0. InvApproxRegs; SimplVM; auto.
+  apply make_divuimm_correct; auto.
+- (* modu *)
+  assert (e#r2 = Vint n2). clear H0. InvApproxRegs; SimplVM; auto.
+  apply make_moduimm_correct; auto.
+- (* and 1 *)
+  rewrite Val.and_commut in H0. InvApproxRegs; SimplVM; inv H0. apply make_andimm_correct; auto.
+- (* and 2 *)
+  InvApproxRegs; SimplVM; inv H0. apply make_andimm_correct; auto.
+- (* andimm *)
+  inv H; inv H0. apply make_andimm_correct; auto.
+- (* or 1 *)
+  rewrite Val.or_commut in H0. InvApproxRegs; SimplVM; inv H0. apply make_orimm_correct; auto.
+- (* or 2 *)
+  InvApproxRegs; SimplVM; inv H0. apply make_orimm_correct; auto.
+- (* xor 1 *)
+  rewrite Val.xor_commut in H0. InvApproxRegs; SimplVM; inv H0. apply make_xorimm_correct; auto.
+- (* xor 2 *)
+  InvApproxRegs; SimplVM; inv H0. apply make_xorimm_correct; auto.
+- (* shl *)
+  InvApproxRegs; SimplVM; inv H0. apply make_shlimm_correct; auto.
+- (* shr *)
+  InvApproxRegs; SimplVM; inv H0. apply make_shrimm_correct; auto.
+- (* shru *)
+  InvApproxRegs; SimplVM; inv H0. apply make_shruimm_correct; auto.
+- (* cond *)
+  inv H0. apply make_cmp_correct; auto.
+- (* mulf 1 *)
+  InvApproxRegs; SimplVM; inv H0. rewrite <- H2. apply make_mulfimm_correct; auto.
+- (* mulf 2 *)
+  InvApproxRegs; SimplVM; inv H0. fold (Val.mulf (Vfloat n1) e#r2).
+  rewrite <- H2. apply make_mulfimm_correct_2; auto.
+- (* mulfs 1 *)
+  InvApproxRegs; SimplVM; inv H0. rewrite <- H2. apply make_mulfsimm_correct; auto.
+- (* mulfs 2 *)
+  InvApproxRegs; SimplVM; inv H0. fold (Val.mulfs (Vsingle n1) e#r2).
+  rewrite <- H2. apply make_mulfsimm_correct_2; auto.
+- (* default *)
+  exists v; auto.
+Qed.
+
+Lemma addr_strength_reduction_correct:
+  forall addr args vl res,
+  vl = map (fun r => AE.get r ae) args ->
+  eval_addressing ge (Vptr sp Ptrofs.zero) addr e##args = Some res ->
+  let (addr', args') := addr_strength_reduction addr args vl in
+  exists res', eval_addressing ge (Vptr sp Ptrofs.zero) addr' e##args' = Some res' /\ Val.lessdef res res'.
+Proof.
+  intros until res. unfold addr_strength_reduction.
+  destruct (addr_strength_reduction_match addr args vl); simpl;
+  intros VL EA; InvApproxRegs; SimplVM; try (inv EA).
+- simpl. rewrite Genv.shift_symbol_address. econstructor; split; eauto.
+  inv H0; simpl; auto.
+- rewrite Ptrofs.add_zero_l. econstructor; split; eauto.
+  change (Vptr sp (Ptrofs.add n1 n)) with (Val.offset_ptr (Vptr sp n1) n).
+  inv H0; simpl; auto.
+- exists res; auto.
+Qed.
+
+End STRENGTH_REDUCTION.
